pcuic/theories/PCUICContexts.v
@@ -2,7 +2,7 @@
 From MetaCoq.Template Require Import config utils.
 From Coq Require Import CRelationClasses ProofIrrelevance.
 From MetaCoq.Template Require Import config Universes utils BasicAst.
-From MetaCoq.PCUIC Require Import PCUICAst PCUICAstUtils PCUICInduction
+From MetaCoq.PCUIC Require Import PCUICAst PCUICAstUtils PCUICTactics PCUICInduction
      PCUICReflect PCUICLiftSubst PCUICUnivSubst PCUICTyping
      PCUICEquality
      PCUICInversion PCUICCumulativity PCUICReduction
