pcuic/theories/Typing/PCUICInstTyp.v
@@ -1,7 +1,7 @@
 (* Distributed under the terms of the MIT license. *)
 From Coq Require Import Morphisms.
 From MetaCoq.Template Require Import config utils.
-From MetaCoq.PCUIC Require Import PCUICAst PCUICAstUtils PCUICCases PCUICInduction
+From MetaCoq.PCUIC Require Import PCUICAst PCUICAstUtils PCUICTactics PCUICCases PCUICInduction
   PCUICLiftSubst PCUICUnivSubst
   PCUICTyping PCUICReduction PCUICCumulativity 
   PCUICEquality PCUICGlobalEnv PCUICClosed PCUICClosedConv PCUICClosedTyp PCUICEquality PCUICWeakeningEnvConv PCUICWeakeningEnvTyp
